verify a mid impl of tseitin

LeanSAT/Encode/Tseitin.lean
@@ -2,397 +2,235 @@ import LeanSAT.Encode.VEncCNF
 
 /-! ## Tseitin Transform
 
-This file implements an optimized version of the Tseitin transformation
-from arbitrary formulas to CNF.
+This file implements a lightly optimized Tseitin encoding
+of arbitrary `PropForm` formulas into CNF.
 
-Formulas are first normalized, pushing negations down to the atoms
-and collecting nested ands/ors into a single multi-child and/or.
+The formula is put into negation normal form first,
+and top-level ∧ / top-level ∨ are collected into one
+formula/clause respectively.
 -/
 
 namespace LeanSAT.Encode.Tseitin
 
 open Model
 
-inductive ReducedForm (L : Type u) : Bool → Type u
-| and (fs : Array (ReducedForm L false)) : ReducedForm L true
-| or  (fs : Array (ReducedForm L true )) : ReducedForm L false
-| lit (l : L) : ReducedForm L b
-deriving Repr
+inductive NegNormForm (L : Type u)
+| and (a b : NegNormForm L)
+| or (a b : NegNormForm L)
+| tr | fls
+| lit (l : L)
+deriving Repr, DecidableEq
 
-private def ReducedForm.disjuncts : ReducedForm L false → Array (ReducedForm L true)
-| .or fs => fs
-| .lit l => #[.lit l]
+namespace NegNormForm
 
-private def ReducedForm.conjuncts : ReducedForm L true → Array (ReducedForm L false)
-| .and fs => fs
-| .lit l => #[.lit l]
+variable [LitVar L ν]
 
-def const (val : Bool) : ReducedForm L b :=
-  match b, val with
-  | true , true  => .and #[]
-  | true , false => .and #[.or #[]]
-  | false, true  => .or #[.and #[]]
-  | false, false => .or #[]
-
-@[simp] noncomputable def reduceSize : PropForm L → Nat
-| .var _ | .tr | .fls => 1
-| .neg x => 1 + reduceSize x
-| .conj x y | .disj x y => 1 + reduceSize x + reduceSize y
-| .impl x y   => 3 + reduceSize x + reduceSize y
-| .biImpl x y => 8 + 2 * (reduceSize x + reduceSize y)
-
-@[simp] theorem reduceSize_pos : reduceSize f > 0 := by
-  cases f <;> simp
-
-variable {L : Type u} {ν : Type v} [LitVar L ν] in
-mutual
-
-/-- `reduce φ b` returns a formula equivalent
-to `φ` if `b = true` or `¬φ` if `b = false`. -/
-def reduce : PropForm ν → Bool → ReducedForm L b
-| .neg f, neg =>
-    reduce f (!neg)
-| .var l, neg =>
-    .lit <| LitVar.mkLit _ l (!neg)
-| .tr, neg =>
-    const (!neg)
-| .fls, neg =>
-    const ( neg)
-| .conj x y, neg =>
-    if neg
-    then reduceDisj x y true
-    else reduceConj x y false
-| .disj x y, neg =>
-    if neg
-    then reduceConj x y true
-    else reduceDisj x y false
-| .impl h c, neg =>
-    reduce (.disj c (.neg h)) neg
-| .biImpl l r, neg =>
-    reduce (.conj (.impl l r) (.impl r l)) neg
-
-def reduceConj (x y : PropForm ν) (neg : Bool) : ReducedForm L b :=
-  let blah := .and <| (reduce x neg).conjuncts ++ (reduce y neg).conjuncts
-  match b with
-  | true  => blah
-  | false => .or #[blah]
-
-def reduceDisj (x y : PropForm ν) (neg : Bool) : ReducedForm L b :=
-  let blah := .or <| (reduce x neg).disjuncts ++ (reduce y neg).disjuncts
-  match b with
-  | true  => .and #[blah]
-  | false => blah
-end
-termination_by
-  reduce f neg => reduceSize f
-  reduceConj x y neg => reduceSize x + reduceSize y
-  reduceDisj x y neg => reduceSize x + reduceSize y
-
-def ReducedForm.toPropFun [LitVar L V] (r : ReducedForm L b) : PropFun V :=
+def toPropFun (r : NegNormForm L) : PropFun ν :=
   match r with
-  | and fs =>
-    let fs' := fs.attach.map (fun ⟨x,_h⟩ => ReducedForm.toPropFun x)
-    PropFun.all fs'.toList
-  | or fs  =>
-    let fs' := fs.attach.map (fun ⟨x,_h⟩ => ReducedForm.toPropFun x)
-    PropFun.any fs'.toList
-  | lit l => LitVar.toPropFun l
+  | .and a b => a.toPropFun ⊓ b.toPropFun
+  | .or a b  => a.toPropFun ⊔ b.toPropFun
+  | .lit l => LitVar.toPropFun l
+  | .tr => ⊤
+  | .fls => ⊥
 
-@[simp] theorem const_toPropFun [LitVar L ν]
-  : (const b1 : ReducedForm L b2).toPropFun = if b1 then ⊤ else ⊥
-  := by
-  ext τ
-  cases b1 <;> cases b2 <;> (
-    simp [const]
-    simp [ReducedForm.toPropFun, Array.mem_def, Array.attach]
-  )
+def const (val : Bool) : NegNormForm L :=
+  match val with
+  | true  => .tr
+  | false => .fls
 
-theorem ReducedForm.conjuncts_toPropFun [LitVar L ν] (r : ReducedForm L true)
-  : r.toPropFun = (PropFun.all (r.conjuncts.toList.map toPropFun)) :=
-  match r with
-  | .and rs => by ext τ; simp [conjuncts, Array.mem_def, Array.attach, toPropFun]
-  | .lit l => by ext τ; simp [conjuncts, Array.mem_def]; rfl
+@[simp] theorem const_toPropFun
+  : (const b : NegNormForm L).toPropFun = if b then ⊤ else ⊥
+  := by ext τ; cases b <;> simp [const, toPropFun]
 
-theorem ReducedForm.disjuncts_toPropFun [LitVar L ν] (r : ReducedForm L false)
-  : r.toPropFun = (PropFun.any (r.disjuncts.toList.map toPropFun)) :=
-  match r with
-  | .or rs => by ext τ; simp [disjuncts, Array.mem_def, Array.attach, toPropFun]
-  | .lit l => by ext τ; simp [disjuncts, Array.mem_def]; rfl
+def ofPropForm (neg : Bool) : PropForm ν → NegNormForm L
+| .tr => const (!neg)
+| .fls => const neg
+| .var v => .lit <| LitVar.mkLit _ v (!neg)
+| .neg f => ofPropForm (!neg) f
+| .conj a b =>
+  if neg then
+    .or (ofPropForm neg a) (ofPropForm neg b)
+  else
+    .and (ofPropForm neg a) (ofPropForm neg b)
+| .disj a b =>
+  if neg then
+    .and (ofPropForm neg a) (ofPropForm neg b)
+  else
+    .or (ofPropForm neg a) (ofPropForm neg b)
+| .impl a b =>
+  if neg then
+    .and (ofPropForm false a) (ofPropForm true b)
+  else
+    .or (ofPropForm true a) (ofPropForm false b)
+| .biImpl a b =>
+  if neg then
+    .or
+      (.and (ofPropForm false a) (ofPropForm true b))
+      (.and (ofPropForm false b) (ofPropForm true a))
+  else
+    .and
+      (.or (ofPropForm true a) (ofPropForm false b))
+      (.or (ofPropForm true b) (ofPropForm false a))
 
-#eval show ReducedForm ILit true from
-  reduce (.biImpl (.var 1) (.conj (.biImpl (.var 2) (.var 3)) (.biImpl (.var 4) (.var 2)))) true
+theorem toPropFun_ofPropForm [LawfulLitVar L ν] (f : PropForm ν)
+  : toPropFun (L := L) (ofPropForm neg f) =
+      if neg then ⟦.neg f⟧ else ⟦f⟧ := by
+  induction f generalizing neg <;>
+    -- we ♥ aesop
+    aesop (add norm 1 simp ofPropForm)
+          (add norm 1 simp toPropFun)
+          (add norm 1 simp himp_eq)
+          (add norm 1 simp PropFun.biImpl_eq_impls)
 
-#exit
+def cleanup : NegNormForm L → NegNormForm L
+| tr => .tr
+| fls => .fls
+| lit l => .lit l
+| and a b =>
+  let a := cleanup a
+  let b := cleanup b
+  match a, b with
+  | .tr, x
+  | x, .tr => x
+  | .fls, _
+  | _, .fls => .fls
+  | _, _ => .and a b
+| or  a b =>
+  let a := cleanup a
+  let b := cleanup b
+  match a, b with
+  | .tr, _
+  | _, .tr => .tr
+  | .fls, x
+  | x, .fls => x
+  | _, _ => .or a b
 
-/- TODO: This proof is really slow...
-
-JG: investigated this a bit more, it seems like the proof is not actually
-that slow, mutual blocks are just hard...
--/
-set_option maxHeartbeats 500000 in
-open PropFun in
-variable {L : Type u} {ν : Type v} [LitVar L ν] [LawfulLitVar L ν] in
-mutual
-def reduce_toPropFun (f : PropForm ν) (neg : Bool)
-  : (reduce f neg : ReducedForm L b).toPropFun = ⟦ if neg then .neg f else f ⟧ :=
-  match f with
-  | .neg f =>
-      have := reduce_toPropFun f (!neg)
-      by
-        simp [reduce]; rw [this]; cases neg <;> simp
-  | .var l =>
-      by
-        simp [reduce]
-        cases neg <;> simp [ReducedForm.toPropFun, LitVar.toPropFun]
-  | .tr =>
-      by
-        simp [reduce]
-        cases neg <;> simp
-  | .fls =>
-      by
-        simp [reduce]
-        cases neg <;> simp
-  | .conj x y =>
-      have h1 := reduceDisj_toPropFun (b := b) x y true
-      have h2 := reduceConj_toPropFun (b := b) x y false
-      by
-        simp [reduce]; cases neg <;> simp <;> (first | rw [h1] | rw [h2]) <;> simp
-  | .disj x y =>
-      have h1 := reduceConj_toPropFun (b := b) x y true
-      have h2 := reduceDisj_toPropFun (b := b) x y false
-      by
-        simp [reduce]; cases neg <;> simp <;> (first | rw [h1] | rw [h2]) <;> simp
-  | .impl h c =>
-      have h' := reduce_toPropFun (b := b) (.disj c (.neg h)) neg
-      by
-        unfold reduce; rw [h']; clear h'
-        cases neg <;> simp [BooleanAlgebra.sdiff_eq, BooleanAlgebra.himp_eq]
-  | .biImpl l r =>
-      have h' := reduce_toPropFun (b := b) (.conj (.impl l r) (.impl r l)) neg
-      by
-        unfold reduce; rw [h']; clear h'
-        cases neg <;> simp [biImpl_eq_impls, BooleanAlgebra.sdiff_eq, BooleanAlgebra.himp_eq]
-
-def reduceConj_toPropFun (x y : PropForm ν) (neg : Bool)
-  : (reduceConj x y neg : ReducedForm L b).toPropFun =
-      ⟦ if neg then .neg (.disj x y) else (.conj x y) ⟧
-  := by
-  have h1 := reduce_toPropFun (b := true) x neg
-  have h2 := reduce_toPropFun (b := true) y neg
-  ext τ
-  have := congrArg (τ ⊨ ·) <| ReducedForm.conjuncts_toPropFun (L := L) (reduce x neg)
-  rw [h1] at this
-  have := congrArg (τ ⊨ ·) <| ReducedForm.conjuncts_toPropFun (L := L) (reduce y neg)
-  rw [h2] at this
-  clear h1 h2
-  cases b <;> (
-    simp [reduceConj]
-    simp [ReducedForm.toPropFun, Array.mem_def, Array.attach] at *
-    aesop
-  )
-
-
-def reduceDisj_toPropFun (x y : PropForm ν) (neg : Bool)
-  : (reduceDisj x y neg : ReducedForm L b).toPropFun =
-    ⟦ if neg then .neg (.conj x y) else .disj x y ⟧
-  := by
-  have h1 := reduce_toPropFun (b := false) x neg
-  have h2 := reduce_toPropFun (b := false) y neg
-  ext τ
-  have := congrArg (τ ⊨ ·) <| ReducedForm.disjuncts_toPropFun (L := L) (reduce x neg)
-  rw [h1] at this
-  have := congrArg (τ ⊨ ·) <| ReducedForm.disjuncts_toPropFun (L := L) (reduce y neg)
-  rw [h2] at this
-  clear h1 h2
-  cases b <;> (
-    simp [reduceDisj]
-    simp [ReducedForm.toPropFun, Array.mem_def, Array.attach] at *
-    cases neg <;> (
-      simp_all; clear this; clear this
-      generalize ReducedForm.disjuncts _ = xr
-      generalize ReducedForm.disjuncts _ = yr
-      cases xr; cases yr
-      aesop
-    )
-  )
-end
-termination_by
-  reduce_toPropFun f neg => reduceSize f
-  reduceConj_toPropFun x y neg => reduceSize x + reduceSize y
-  reduceDisj_toPropFun x y neg => reduceSize x + reduceSize y
+@[simp] theorem toPropFun_cleanup [LawfulLitVar L ν] (f : NegNormForm L)
+  : toPropFun (L := L) (cleanup f) = toPropFun f := by
+  apply Eq.symm -- otherwise aesop rewrites in the wrong direction
+  induction f <;>
+    -- we ♥ aesop
+    aesop (add norm 1 simp ofPropForm)
+          (add norm 1 simp toPropFun)
+          (add norm 1 simp cleanup)
 
 /-
-def ReducedForm.map [LitVar L V] [LitVar L' V'] (f : V → V') : ReducedForm L b → ReducedForm L' b
-| lit l => .lit (LitVar.mkLit _ (f <| LitVar.toVar l) (LitVar.polarity l))
-| and rs => .and (rs.attach.map (fun ⟨r,_⟩ => map f r))
-| or rs => .or (rs.attach.map (fun ⟨r,_⟩ => map f r))
+structure CNFish (L : Type u) where
+  clauses : Array (Array (NegNormForm L))
+deriving Repr
 
-@[simp]
-def ReducedForm.toPropFun_map [LitVar L V] [LawfulLitVar L V] [LitVar L' V'] [LawfulLitVar L' V']
-          (f : V → V') (r : ReducedForm L b)
-      : toPropFun (map (L' := L') f r) = (toPropFun r).map f :=
-  match r with
-  | .lit l => by
-    simp [map, toPropFun, LitVar.toPropFun]
-    split <;> simp_all
-  | .and rs =>
-    have ih : ∀ r ∈ rs, toPropFun (map f r) = (toPropFun r).map f :=
-      fun rf h => toPropFun_map f rf
-    by
-    simp [map, toPropFun]
-    ext τ
-    simp
-    constructor
-    · rintro h _ rf hrf _ rfl
-      have := h (toPropFun (map f rf)) _ rf ⟨?_,rfl⟩ ?_ rfl
-      · rw [ih rf hrf] at this; simpa using this
-      · use hrf
-      · simp [Array.mem_def, Array.attach]; use rf; simpa [Array.mem_def] using hrf
-    · rintro h _ _ rf ⟨⟨hrf,h1⟩,rfl⟩ _ rfl
-      rw [ih rf hrf]
-      simp
-      apply h
-      · apply h1
-      · rfl
-      · apply hrf
-  | .or rs =>
-    have ih : ∀ r ∈ rs, toPropFun (map f r) = (toPropFun r).map f :=
-      fun rf h => toPropFun_map f rf
-    by
-    simp [map, toPropFun]
-    ext τ
-    simp
-    constructor
-    · rintro ⟨_,⟨⟨rf,⟨hrf,h1⟩,rfl⟩,h2⟩,h4⟩
-      rw [ih rf hrf] at h4; simp at h4
-      refine ⟨_,⟨hrf,h1⟩,h4⟩
-    · rintro ⟨rf,⟨hrf,h1⟩,h2⟩
-      rw [← PropFun.satisfies_map, ← ih rf hrf] at h2
-      refine ⟨_,⟨⟨rf,⟨hrf,h1⟩,rfl⟩,?_⟩,h2⟩
-      simp [Array.mem_def, Array.attach]; use rf; simpa [Array.mem_def] using hrf
+def CNFish.toPropFun [LawfulLitVar L ν] (C : CNFish L) : PropFun ν :=
+  .all <|
+    C.clauses.toList.map (fun clause =>
+      PropFun.any (ν := ν) <|
+        clause.toList.map NegNormForm.toPropFun)
+
+def toCNFish (f : NegNormForm L) : CNFish L :=
+  ⟨ands f⟩
+where
+  ands (f : NegNormForm L) : Array (Array (NegNormForm L)) :=
+    match f with
+    | .and a b => ands a ++ ands b
+    | _ => #[ors f]
+  ors (f : NegNormForm L) : Array (NegNormForm L) :=
+    match f with
+    | .or a b => ors a ++ ors b
+    | _ => #[f]
+
+@[simp] theorem toPropForm_toCNFish [LawfulLitVar L ν] (f : NegNormForm L)
+  : (toCNFish f).toPropFun = f.toPropFun := by
+  sorry --TODO make use of this
 -/
 
+end NegNormForm
+
+open VEncCNF
+attribute [local simp] NegNormForm.toPropFun
+
+/-- Tseitin encoding in the general case creates temporaries for each clause -/
+def encodeNNF_mkDefs [LitVar L ν] [LitVar L' ν'] [LawfulLitVar L ν] [DecidableEq ν] [Fintype ν]
+        (t : ν) (emb : ν' ↪ ν) (f : NegNormForm L')
+  : VEncCNF L Unit (.biImpl (.var t) (f.toPropFun.map emb)) :=
+  match f with
+  | .tr =>
+      addClause #[LitVar.mkPos t]
+      |>.mapProp (by simp [Clause.toPropFun, PropFun.any])
+  | .fls =>
+      addClause #[LitVar.mkNeg t]
+      |>.mapProp (by simp [Clause.toPropFun, PropFun.any])
+  | .lit l =>
+      biImpl (LitVar.mkPos t) (LitVar.map emb l)
+      |>.mapProp (by simp)
+  | .and a b =>
+      withTemps 2 (
+        seq
+          (encodeNNF_mkDefs (.inr 0) (emb.trans ⟨Sum.inl,Sum.inl_injective⟩) a)
+          (seq
+          (encodeNNF_mkDefs (.inr 1) (emb.trans ⟨Sum.inl,Sum.inl_injective⟩) b)
+          (defConj (.var t) #[.temp 0, .temp 1]))
+      ) |>.mapProp (by
+        ext τ; simp
+        constructor
+        case a.mp =>
+          aesop
+        case a.mpr =>
+          intro h
+          open PropFun in
+          use fun
+            | .inl v => τ v
+            | .inr 0 => τ.map emb ⊨ a.toPropFun
+            | .inr 1 => τ.map emb ⊨ b.toPropFun
+          aesop)
+  | .or a b =>
+      withTemps 2 (
+        seq
+          (encodeNNF_mkDefs (.inr 0) (emb.trans ⟨Sum.inl,Sum.inl_injective⟩) a)
+          (seq
+          (encodeNNF_mkDefs (.inr 1) (emb.trans ⟨Sum.inl,Sum.inl_injective⟩) b)
+          (defDisj (.var t) #[.temp 0, .temp 1]))
+      ) |>.mapProp (by
+        ext τ; simp
+        constructor
+        case a.mp =>
+          aesop
+        case a.mpr =>
+          intro h
+          open PropFun in
+          use fun
+            | .inl v => τ v
+            | .inr 0 => τ.map emb ⊨ a.toPropFun
+            | .inr 1 => τ.map emb ⊨ b.toPropFun
+          aesop)
+
+def encodeNNF [LitVar L ν] [LawfulLitVar L ν] [DecidableEq ν] [Fintype ν]
+        (f : NegNormForm L) : VEncCNF L Unit f.toPropFun :=
+  match f with
+  | .tr => VEncCNF.pure () -- type matches by rfl
+  | .fls => addClause #[]  -- type matches by rfl
+  | .lit l => addClause #[l] |>.mapProp (by simp [Clause.toPropFun, PropFun.any])
+  | .and a b =>
+    seq (encodeNNF a) (encodeNNF b) -- type matches by rfl
+  | .or a b =>
+    withTemps 2 (
+        seq (encodeNNF_mkDefs (.inr 0) ⟨Sum.inl,Sum.inl_injective⟩ a)
+      ( seq (encodeNNF_mkDefs (.inr 1) ⟨Sum.inl,Sum.inl_injective⟩ b)
+            (addClause #[.temp 0, .temp 1]))
+    ) |>.mapProp (by
+      apply Eq.symm -- otherwise aesop rewrites in the wrong direction
+      ext τ
+      simp [Clause.toPropFun]
+      open PropFun in
+      constructor
+      case a.mp =>
+        intro h
+        use fun | .inl v => τ v | .inr 0 => τ ⊨ a.toPropFun | .inr 1 => τ ⊨ b.toPropFun
+        aesop
+      case a.mpr =>
+        aesop
+      )
 
 noncomputable def tseitin [LitVar L V] [LawfulLitVar L V] [DecidableEq V] [Fintype V]
       (f : PropForm V) : VEncCNF L Unit ⟦f⟧ :=
-  let red : ReducedForm L true := reduce f false
-  let conjs := red.conjuncts
-  sorry
-  /- for_all conjs (fun conj : ReducedForm L false =>
-    withTemps conj.disjuncts.size (
-      let temps := List.fins conj.disjuncts.size |>.toArray
-      for_all temps (fun i =>
-        aux (L := EncCNF.WithTemps L conj.disjuncts.size) (V := V ⊕ Fin conj.disjuncts.size)
-          (Sum.inr i)
-          (ReducedForm.map Sum.inl conj.disjuncts[i]))
-    )
-  )
-  |> mapProp (by
-    sorry
-  ) -/
-where
-  aux {b} (t : V) (f : ReducedForm L b)
-      : VEncCNF L Unit (.biImpl (.var t) (f.toPropFun)) :=
-    sorry
-/-
-    match h : f with
-    | .lit l =>
-      seq (addClause #[.var l, LitVar.negate <| .temp 0])
-          (addClause #[LitVar.negate <| .var l, .temp 0])
-      |> mapProp (by
-        subst b; simp at h; subst f
-        ext τ
-        simp [Clause.satisfies_iff, LitVar.satisfies_iff, ReducedForm.toPropFun]
-        generalize τ _ = x; generalize τ _ = y; generalize LitVar.polarity l = z
-        cases y <;> cases z <;> simp)
-    | .and fs =>
-      --withTemps fs.size (
-      --  let temps := List.fins fs.size |>.map EncCNF.WithTemps.temp
-      --  seq
-      --    -- temp i ↔ fs[i]
-      --    (forIn temps sorry)
-      --  <| seq
-      --    -- temp 0 ↔ ⋀ᵢ temp i
-      --    (forIn temps (fun i => addClause #[ sorry, fs[i]]))
-      --    (assuming temps <| addClause #[EncCNF.WithTemps.temp 0])
-      --) |> mapProp
-      sorry
-    | .or fs => sorry
-      --do
-      --let ls ← fs.subtypeSize.mapM (fun ⟨f,h⟩ =>
-      --  have := Nat.le_trans h (Nat.le_add_left _ 1)
-      --  aux f)
-      --let t ← mkTemp
-      ---- t ↔ ⋁ ls
-      --assuming #[t] <| addClause ls
-      --for l in ls do
-      --  addClause #[-l, t]
-      --return t
--/
-
-open EncCNF in
-def encodeAux {L V L' V' : Type} [LitVar L V] [LitVar L' V'] [Fintype V]
-      (t : V) (f : ReducedForm L' b) (emb : L' ↪ L) :
-    EncCNF L (Option L') := do
-  match f with
-  | .lit l => return some l
-  | .and fs =>
-    withTemps fs.size (do
-    let fs' : Array (L ⊕ Fin fs.size) ←
-      Array.ofFn (n := fs.size) id |>.mapM (fun i => do
-        match ←
-          encodeAux (.inr i) (fs[i] : ReducedForm L' _)
-            ⟨ (.var <| emb ·)
-            , by intro l1 l2 h; simp [WithTemps.var] at h; have := Sum.inl_injective h; simp_all⟩
-        with
-        | none => return .inr i
-        | some l => return .inl (emb l))
-    -- ∀ i, t → fs[i]
-    for f in fs' do
-      sorry
-    -- ⋀i fs[i] → t
-    addClause #[]
-    return none
-    )
-  | .or fs => sorry
-
-def encode [LitVar L V] (f : PropForm V) : EncCNF L Unit :=
-  let red : ReducedForm L true := reduce f false
-  let conjs := red.conjuncts
-where
-toplevel : Formula.NegNorm → EncCNF Unit
-  | .lit l => addClause l
-  | .and fs => newCtx "and." do
-    for (i,⟨f,h⟩) in fs.subtypeSize.enum do
-      have := Nat.le_trans h (Nat.le_add_left _ 1)
-      newCtx s!"[{i}]." <| toplevel f
-  | .or fs => newCtx "or." do
-    let ls ← fs.enum.mapM (fun (i,f) => newCtx s!"[{i}]." <| aux f)
-    addClause ls
-aux : Formula.NegNorm → EncCNF Literal
-  | .lit l => pure l
-  | .and fs => newCtx "and." do
-    let ls : List Literal ← fs.subtypeSize.enum.mapM (fun (i, ⟨f,h⟩) =>
-      have := Nat.le_trans h (Nat.le_add_left _ 1)
-      newCtx s!"[{i}]." <| aux f)
-    let t ← mkTemp
-    -- t ↔ ⋀ ls
-    for l in ls do
-      addClause (¬ t ∨ l)
-    addClause (ls.map (·.not) ∨ t)
-    return t
-  | .or  fs => newCtx "or." do
-    let ls ← fs.subtypeSize.enum.mapM (fun (i, ⟨f,h⟩) =>
-      have := Nat.le_trans h (Nat.le_add_left _ 1)
-      newCtx s!"[{i}]." <| aux f)
-    let t ← mkTemp
-    -- t ↔ ⋁ ls
-    addClause (¬ t ∨ ls)
-    for l in ls do
-      addClause (¬l ∨ t)
-    return t
-termination_by
-  toplevel f => f
-  aux f => f
-
-end Tseitin
+  let nnf : NegNormForm L := (NegNormForm.ofPropForm false f).cleanup
+  encodeNNF nnf
+  |>.mapProp (by simp [NegNormForm.toPropFun_ofPropForm])
